Alternative syntax (without context) easier to use

theories/systemF_alt.v
@@ -80,6 +80,8 @@ End Relation.
   | v_abs : forall x t1, is_val (expr_abs x t1)
   | v_tabs : forall t1, is_val (expr_tabs t1).
 
+  Hint Constructors is_val : core.
+
 
   (** Equality  *)
   (* Lemma to_of_val v : to_val (of_val v) = Some v. *)
@@ -246,54 +248,53 @@ End Relation.
     Δ;Γ ⊢ e _ ∈ <{ [ α := τ1 ] τ2 }>
   where "Δ ; Γ '⊢' t '∈' T" := (typing_judgment Δ Γ t T).
 
+  Hint Constructors typing_judgment : core.
+
   Notation "( x )" := x (in custom sf, x at level 99).
-  Reserved Notation "t '-h->' t'" (at level 60).
-  Inductive pure_step : expr -> expr -> Prop :=
-  | step_fst : forall v1 v2,
-    is_val v1 ->
-    is_val v2 ->
-    <{ fst ⟨ v1, v2 ⟩ }> -h->  <{ v1 }>
-  | step_snd : forall v1 v2,
-    is_val v1 ->
-    is_val v2 ->
-    <{ snd ⟨ v1, v2 ⟩ }> -h->  <{ v2 }>
-  | step_lam : forall x e v,
-    is_val v ->
-    <{ (λ x, e) v }> -h->  <{ [x / v]e }>
-  | step_tlam : forall e,
-    <{ (Λ e) _ }> -h->  <{ e }>
-  where "t '-h->' t'" := (pure_step t t').
-
-  Inductive ectx : Type :=
-  | EmptyCtx : ectx
-  | FstCtx : ectx -> ectx
-  | SndCtx : ectx -> ectx
-  | LPairCtx : ectx -> expr -> ectx
-  | RPairCtx : ectx -> val -> ectx
-  | LAppCtx : ectx -> expr -> ectx
-  | RAppCtx : ectx -> val -> ectx
-  | TAppCtx : ectx -> ectx.
-
-  Fixpoint fill (c : ectx) (e : expr) : expr :=
-    match c with
-    | EmptyCtx => e
-    | FstCtx K => expr_fst (fill K e)
-    | SndCtx K => expr_snd (fill K e)
-    | LPairCtx K t => expr_pair (fill K e) t
-    | RPairCtx K v => expr_pair (of_val v) (fill K e)
-    | LAppCtx K t => expr_app (fill K e) t
-    | RAppCtx K v => expr_app (of_val v) (fill K e)
-    | TAppCtx K => expr_tapp (fill K e)
-    end.
-
   Reserved Notation "t '~>' t'" (at level 60).
-  Inductive step e1 e2 : Prop :=
-  | Step K e1' e2' :
-    e1 = fill K e1' ->
-    e2 = fill K e2' ->
-    e1' -h-> e2' ->
-    e1 ~> e2
-  where "e1 '~>' e2" := (step e1 e2).
+  Inductive step : expr -> expr -> Prop :=
+  | step_fst_red : forall v1 v2,
+    is_val v1 ->
+    is_val v2 ->
+    <{ fst ⟨ v1, v2 ⟩ }> ~>  <{ v1 }>
+  | step_snd_red : forall v1 v2,
+    is_val v1 ->
+    is_val v2 ->
+    <{ snd ⟨ v1, v2 ⟩ }> ~>  <{ v2 }>
+  | step_lam_red : forall x e v,
+    is_val v ->
+    <{ (λ x, e) v }> ~>  <{ [x / v]e }>
+  | step_tlam_red : forall e,
+    <{ (Λ e) _ }> ~>  <{ e }>
+  | step_fst : forall e e',
+    e ~> e' ->
+    <{ fst e }> ~>  <{ fst e' }>
+
+  | step_snd : forall e e',
+    e ~> e' ->
+    <{ snd e }> ~>  <{ snd e' }>
+
+  | step_pairL : forall e1 e1' e2,
+    e1 ~> e1' ->
+    <{ ⟨ e1, e2 ⟩ }> ~>  <{ ⟨ e1', e2 ⟩  }>
+
+  | step_pairR : forall v e e',
+    is_val v ->
+    e ~> e' ->
+    <{ ⟨ v, e ⟩ }> ~>  <{ ⟨ v, e' ⟩  }>
+
+  | step_lam_head : forall f f' e,
+    f ~> f' ->
+    <{ f e }> ~>  <{ f' e }>
+  | step_lam_arg : forall f e e',
+    is_val f ->
+    e ~> e' ->
+    <{ f e }> ~>  <{ f e' }>
+  | step_tlam_head : forall e e',
+    e ~> e' ->
+    <{ e _ }> ~>  <{ e' _ }>
+  where "t '~>' t'" := (step t t').
+  Hint Constructors step : core.
 
   Definition mstep := star expr step.
   Notation "t '~>*' t'" := (mstep t t') (at level 60).
@@ -301,16 +302,11 @@ End Relation.
   (* Definition reducible (e : expr) := *)
   (*   ∃ e', step e e'. *)
 
-  Lemma fill_empty e : fill EmptyCtx e = e.
-  Proof. done. Qed.
-
   (** Examples *)
   Goal <{ (λ x , x) tt }> ~>* <{tt}>.
   Proof.
     eapply star_one.
-    eapply (Step _ _ EmptyCtx) ;
-      [ done | done |].
-    apply step_lam.
+    apply step_lam_red.
     apply v_unit.
   Qed.
 
@@ -318,63 +314,36 @@ End Relation.
   Proof.
     eapply star_trans with <{ fst ( ⟨ (λ y , tt) tt , (λ y , tt) tt⟩ )}>.
     eapply star_one.
-    eapply (Step _ _ (FstCtx EmptyCtx) ).
-    1,2: simpl; done.
-    eapply step_lam; apply v_unit.
+    eapply step_fst; eapply step_lam_red ; apply v_unit.
 
     eapply star_trans with <{ fst ( ⟨ tt , (λ y , tt) tt⟩ )}>.
     eapply star_one.
-    eapply (Step _ _ (FstCtx (LPairCtx EmptyCtx _)) ).
-    1,2: simpl; done.
-    eapply (step_lam y <{ tt }> ); apply v_unit.
+    eapply step_fst; eapply step_pairL; eapply (step_lam_red y <{ tt }> ); apply v_unit.
 
     eapply star_trans with <{ fst ( ⟨ tt , tt⟩ )}>.
     eapply star_one.
-    eapply (Step _ _ (FstCtx (RPairCtx EmptyCtx val_unit)) ).
-    1,2: simpl;done.
-    eapply (step_lam y <{ tt }> ); apply v_unit.
+    eapply step_fst; eapply step_pairR;[apply v_unit|];
+      eapply (step_lam_red y <{ tt }> ); apply v_unit.
 
     eapply star_one.
-    eapply (Step _ _ EmptyCtx).
-    1,2: simpl; done.
-    apply step_fst; apply v_unit.
+    eapply step_fst_red; apply v_unit.
   Qed.
 
   Lemma identity : forall v e, e = (of_val v) -> <{ (λ x , x) e }> ~>* <{e}>.
   Proof.
     intros v e ->.
     eapply star_one.
-    eapply (Step _ _ EmptyCtx).
-    1,2: done.
-    apply step_lam.
+    apply step_lam_red.
     apply is_val_of_val.
   Qed.
-
 
 Lemma is_val_stuck : forall e e', is_val e -> not (e ~> e').
 Proof.
   intros e e' val_e.
   generalize dependent e'.
   induction e; intros e' step; try inversion val_e;inversion step; subst.
-  - destruct K; subst; simpl in *; try discriminate H.
-    rewrite <- H in H1; inversion H1.
-  - destruct K; subst; simpl in *; try discriminate H3.
-    + rewrite <- H3 in H5.
-      inversion H5.
-    + eapply IHe1 with (fill K e2') in H1.
-      apply H1.
-      inversion H3; subst.
-      eapply (Step _ _ K); auto.
-    + eapply IHe2 with (fill K e2') in H2.
-      apply H2.
-      inversion H3; subst.
-      eapply (Step _ _ K); auto.
-  - destruct K; subst; simpl in *; try discriminate H3.
-    rewrite <- H in H3; inversion H3.
-    all:try discriminate H.
-  - destruct K; subst; simpl in *; try discriminate H3.
-    rewrite <- H in H2; inversion H2.
-    all: try discriminate H.
+  - eapply IHe1 in H1; eapply H1; eauto.
+  - eapply IHe2 in H2; eapply H2; eauto.
 Qed.
 
 Lemma is_val_step : forall e e', is_val e -> e ~>* e' -> e' = e.
@@ -382,3 +351,11 @@ Lemma is_val_step : forall e e', is_val e -> e ~>* e' -> e' = e.
   inversion mstep; subst; auto.
   by apply is_val_stuck in H.
 Qed.
+
+Ltac solve_by_inverts n :=
+  match goal with | H : ?T |- _ =>
+  match type of T with Prop =>
+    solve [
+      inversion H;
+      match n with S (S (?n')) => subst; solve_by_inverts (S n') end ]
+  end end.
