theories/type_safety.v
@@ -1,7 +1,7 @@
 Set Warnings "-notation-overridden,-parsing,-deprecated-hint-without-locality".
 From Coq Require Import Strings.String.
 From stdpp Require Import gmap list.
-From logical_relation Require Import systemF.
+From logical_relation Require Import systemF_alt.
 
 Definition safe (e: expr) :=
   forall e', e ~>* e' ->
@@ -9,48 +9,6 @@ Definition safe (e: expr) :=
 
 
 (* TODO move to systemF.v, because they are properties of the language *)
-Lemma is_val_step : forall e , is_val e -> e ~>* e.
-Admitted.
-
-Lemma is_val_stuck : forall e e', is_val e -> not (e ~> e').
-Proof.
-  intros e e' val_e.
-  generalize dependent e'.
-  induction e; intros e' step; try inversion val_e;inversion step; subst.
-  - destruct K; subst; simpl in *; try discriminate H.
-    rewrite <- H in H1; inversion H1.
-  - destruct K; subst; simpl in *; try discriminate H3.
-    eapply IHe1 with e2' in H1.
-    admit.
-    inversion H3; subst.
-    admit.
-    admit.
-  - destruct K; subst; simpl in *; try discriminate H3.
-    rewrite <- H in H3; inversion H3.
-    all:try discriminate H.
-  - destruct K; subst; simpl in *; try discriminate H3.
-    rewrite <- H in H2; inversion H2.
-    all: try discriminate H.
-Admitted.
-
-Theorem type_safety :
-  forall e t, nil ; empty ⊢ e ∈ t -> safe e.
-Proof.
-  intros.
-  induction H; unfold safe; intros.
-  - (* unit *)
-    left.
-    inversion H; subst.
-    apply v_unit.
-    apply is_val_stuck in H0; [contradiction|].
-    apply v_unit.
-  - (* var *) admit.
-  - (* pair *) admit.
-  - (* fst *) admit.
-  - (* snd *) admit.
-  - (* abs *) admit.
-  - (* app *)
-Abort.
 
 (** Naive Induction --- Fail *)
 Theorem type_safety :
@@ -60,10 +18,7 @@ Proof.
   induction H; unfold safe; intros.
   - (* unit *)
     left.
-    inversion H; subst.
-    apply v_unit.
-    apply is_val_stuck in H0; [contradiction|].
-    apply v_unit.
+    apply is_val_step in H; subst; apply v_unit.
   - (* var *) admit.
   - (* pair *) admit.
   - (* fst *) admit.
@@ -72,6 +27,213 @@ Proof.
   - (* app *)
 Abort.
 
+Lemma is_val_inversion: forall e, is_val e -> ∃ v, e = (of_val v).
+Proof.
+Admitted.
+
 (** Progress and preservation *)
+Theorem progress : ∀ e t,
+  nil; empty ⊢ e ∈ t ->
+       is_val e ∨ ∃ e', e ~> e'.
+Proof.
+  intros.
+  induction H.
+  - (* unit *) left; apply v_unit.
+  - (* var *) admit.
+  - (* pair *)
+    destruct IHtyping_judgment1, IHtyping_judgment2; [left|right..].
+    + apply v_pair;auto.
+    + destruct H2 as [e2' H2].
+      exists <{ ⟨ e1, e2' ⟩ }>.
+      apply is_val_inversion in H1; destruct H1.
+      rewrite H1.
+      apply step_pairR. apply is_val_of_val. auto.
+    + destruct H1 as [e1' H1].
+      exists <{ ⟨ e1', e2 ⟩ }>.
+      apply step_pairL; auto.
+    + destruct H1 as [e1' H1].
+      exists <{ ⟨ e1', e2 ⟩ }>.
+      apply step_pairL; auto.
+  - (* fst *)
+    destruct IHtyping_judgment; right.
+    + inversion H0; try (rewrite <- H1 in H; inversion H).
+    eexists; apply step_fst_red; auto.
+    + destruct H0 as [e' H0].
+      eexists; eapply step_fst; eauto.
+  - (* snd *)
+    destruct IHtyping_judgment; right.
+    + inversion H0; try (rewrite <- H1 in H; inversion H).
+    eexists; apply step_snd_red; auto.
+    + destruct H0 as [e' H0].
+      eexists; eapply step_snd; eauto.
+  - (* abs *) left; apply v_abs.
+  - (* app *)
+    destruct IHtyping_judgment1, IHtyping_judgment2; right.
+    + (* e has to be λ e' *)
+      inversion H1;
+      match goal with
+      | h: ?val = e |- _ => rewrite <- h in H
+      end;subst ; try inversion H.
+      eexists; apply step_lam_red; auto.
+    + destruct H2 as [e2 H2].
+      eexists; eapply step_lam_arg ; eauto.
+    + destruct H1 as [e1 H1].
+      eexists; eapply step_lam_head ; eauto.
+    + destruct H1 as [e1 H1].
+      eexists; eapply step_lam_head ; eauto.
+  - (* tabs *) left; apply v_tabs.
+  - (* tapp *)
+    destruct IHtyping_judgment; right.
+    + (* e has to be Λ e' *)
+      inversion H0;
+      match goal with
+      | h: ?val = e |- _ => rewrite <- h in H
+      end;subst ; try inversion H.
+      eexists; apply step_tlam_red; auto.
+    + destruct H0 as [e' H0].
+      eexists; eapply step_tlam_head; eauto.
+Admitted.
+
+
+Ltac solve_by_inverts n :=
+  match goal with | H : ?T |- _ =>
+  match type of T with Prop =>
+    solve [
+      inversion H;
+      match n with S (S (?n')) => subst; solve_by_inverts (S n') end ]
+  end end.
+
+
+Lemma canonical_form_pair:
+  forall Δ Γ e t1 t2,
+  Δ; Γ ⊢ e ∈ (t1 × t2)
+     -> is_val e
+     -> exists e1 e2, e = <{⟨ e1, e2 ⟩}>.
+Proof.
+  intros * HT val_e.
+  destruct val_e;
+  inversion HT; subst.
+  eexists; eexists; eauto.
+Qed.
+
+Lemma not_free_context_weakening:
+  forall α Γ Γ',
+  Γ ⊆ Γ' →
+  not_free_context α Γ →
+  not_free_context α Γ'.
+Proof.
+  intros.
+  unfold not_free_context in *.
+Admitted.
+
+Lemma weakening : ∀ Δ Δ' Γ Γ' e t,
+  Γ ⊆ Γ' →
+  Δ ; Γ ⊢ e ∈ t →
+  Δ' ; Γ' ⊢ e ∈ t.
+Proof.
+  intros * H Ht.
+  generalize dependent Γ'.
+  generalize dependent Δ'.
+  induction Ht; intros; eauto.
+  - eapply lookup_weaken with (m2 := Γ') in H; eauto.
+  - apply T_Lam. apply IHHt.
+    by apply insert_mono.
+  - apply T_TLam. apply IHHt; eauto.
+    eapply not_free_context_weakening; eauto.
+Qed.
+
+Lemma weakening_empty : ∀ Δ Γ e t, nil ; empty ⊢ e ∈ t -> Δ ; Γ ⊢ e ∈ t.
+Proof.
+  intros.
+  eapply weakening with nil empty.
+  - apply map_empty_subseteq.
+  - done.
+Qed.
+
+Lemma substitution_preserves_typing : ∀ Δ Γ x tx e v t,
+  Δ ; <[x := tx]> Γ ⊢ e ∈ t ->
+  nil ; empty ⊢ v ∈ tx ->
+  Δ ; Γ ⊢ [x/v] e ∈ t.
+Proof.
+  intros * Ht Hv.
+  generalize dependent Γ. generalize dependent t.
+  generalize dependent Δ.
+  induction e; intros * H;
+    (* in each case, we'll want to get at the derivation of H *)
+    inversion H; clear H; subst; simpl; eauto.
+  - (* var *)
+    rename s into y. destruct (x =? y)%string eqn:Heq; subst.
+    + (* x=y *)
+      (* rewrite update_eq in H3. *)
+      (* injection H2 as H2; subst. *)
+      (* apply weakening_empty. assumption. *)
+      admit.
+    + (* x<>y *)
+      apply T_Var.
+      apply eqb_neq in Heq.
+      eapply lookup_insert_ne with (x:=tx) (m := Γ) in Heq.
+      by setoid_rewrite Heq in H3.
+  - (* abs *)
+    admit.
+  - (* tabs *)
+    admit.
+Admitted.
+
+Theorem preservation : ∀ e e' t,
+  nil ; empty ⊢ e ∈ t →
+  e ~> e' →
+  nil ; empty ⊢ e' ∈ t.
+Proof.
+  intros e e' t HTe step.
+  generalize dependent e'.
+  induction HTe; intros.
+  - (* unit *)
+    replace e' with <{ tt }>. apply T_Unit.
+    symmetry; apply (is_val_step <{ tt }> e').
+    apply v_unit.
+    by apply star_one.
+  - (* var *) admit.
+  - (* pair *)
+    inversion step; subst.
+    apply IHHTe1 in H2; apply T_Prod; auto.
+    apply IHHTe2 in H3; apply T_Prod; auto.
+  - (* fst *)
+    inversion step; subst.
+    inversion HTe; subst; auto.
+    apply IHHTe in H0.
+    by eapply T_Fst.
+  - (* snd *)
+    inversion step; subst.
+    inversion HTe; subst; auto.
+    apply IHHTe in H0.
+    by eapply T_Snd.
+  - (* abs *)
+    inversion step; subst.
+  - (* app *)
+    inversion step; subst.
+    + inversion HTe1; subst; auto.
+      admit.
+    + apply IHHTe1 in H2.
+      eapply T_App; eauto.
+    + apply IHHTe2 in H3.
+      eapply T_App; eauto.
+  - (* tabs *)
+    inversion step; subst.
+  - (* tapp *)
+    inversion step; subst.
+    + inversion HTe; subst; auto.
+      admit.
+    + apply IHHTe in H0.
+      eapply T_TApp; eauto.
+Admitted.
+
+Theorem type_safety_progress_preservation:
+  forall e t, nil ; empty ⊢ e ∈ t -> safe e.
+Proof.
+  intros e T HT e' P. induction P.
+  - apply progress in HT. destruct HT; auto.
+  - apply IHP.
+    + apply preservation with (e := a); auto.
+Qed.
 
 (** Logical relation and free theorems --- new files *)
